bloodBag method for is expired is working

dafny/project/BloodBag.dfy
@@ -1,35 +1,126 @@
-module BB {
-    class BloodBag
+class BloodBag
+{
+    ghost var footprint: set<object>;
+    var id: int;
+    var bloodTypeName: string;
+    var donorId: int;
+    var expirayDate: int;
+    var arrivalDate: int;
+    
+    predicate ValidBB()
+    reads this, footprint
     {
-        ghost var footprint: set<object>;
-        var id: int;
-        var bloodType: string;
-        var donorId: int;
-        var expirayDate: string;
-        var arrivalDate: string;
-        
-        predicate ValidBB()
-        reads this, footprint
-        {
-            this in footprint &&
-            id >= 0 &&
-            donorId >= 0 &&
-            (bloodType == "A" || bloodType == "B" || bloodType == "O")
-        }
+        this in footprint &&
+        id >= 0 &&
+        donorId >= 0 &&
+        expirayDate >= 0 &&
+        arrivalDate >= 0 &&
+        (bloodTypeName == "A" || bloodTypeName == "B" || bloodTypeName == "O" || bloodTypeName == "AB" || bloodTypeName == "")
+    }
 
-        constructor(newId: int, newBloodType: string, newDonorId: int, newExpirayDate: string, newArrivalDate: string) 
-        requires newId >= 0
-        requires newDonorId >= 0
-        requires newBloodType == "A" || newBloodType == "B" || newBloodType == "O"
-        ensures fresh(footprint - old(footprint))
-        ensures ValidBB()
-        modifies this, footprint
-        {
-            id := newId;
-            bloodType := newBloodType;
-            donorId := newDonorId;
-            expirayDate := newExpirayDate;
-            arrivalDate := newArrivalDate;
+    constructor()
+    requires ValidBB()
+    ensures ValidBB()
+    ensures fresh(footprint - old(footprint))
+    modifies this, footprint
+    {
+        id := 0;
+        bloodTypeName := "";
+        donorId := 0;
+        expirayDate := 0;
+        arrivalDate := 0;
+        footprint := {this};
+    }
+    
+    method getType() returns(value: string)
+    requires ValidBB() 
+    ensures ValidBB()
+    ensures value == bloodTypeName
+    {
+        value := bloodTypeName;
+    }
+    
+    method setType(BT: string)
+    modifies this, footprint
+    requires ValidBB()
+    requires BT == "A" || BT == "B" || BT == "O" || BT == "AB"
+    ensures fresh(footprint - old(footprint));
+    ensures ValidBB()
+    ensures bloodTypeName == BT
+    {
+        bloodTypeName := BT;
+    }
+    
+    method getDonor() returns(value: int)
+    requires ValidBB() 
+    ensures ValidBB()
+    ensures value == donorId
+    {
+        value := donorId;
+    }
+
+    method setDonor(newDonorId: int) 
+    requires ValidBB()
+    requires newDonorId >= 0
+    ensures ValidBB()
+    ensures fresh(footprint - old(footprint))
+    ensures donorId == newDonorId
+    modifies this, footprint
+    {
+        donorId := newDonorId;
+    }
+
+    method getArrivalDate() returns(value: int)
+    requires ValidBB() 
+    ensures ValidBB()
+    ensures value == arrivalDate
+    {
+        value := arrivalDate;
+    }
+
+    method setArrivalDate(newArrivalDate: int) 
+    requires ValidBB()
+    requires newArrivalDate >= 0
+    ensures ValidBB()
+    ensures arrivalDate == newArrivalDate
+    ensures fresh(footprint - old(footprint))
+    modifies this, footprint
+    {
+        arrivalDate := newArrivalDate;
+    }
+
+    method getExpirayDate() returns (value: int)
+    requires ValidBB()
+    ensures ValidBB()
+    ensures value == expirayDate
+    {
+        value := expirayDate;
+    }
+
+    method setExpirayDate(newExpirayDate: int) 
+    requires ValidBB()
+    requires newExpirayDate >= 0
+    ensures ValidBB()
+    ensures expirayDate == newExpirayDate
+    ensures fresh(footprint - old(footprint))
+    modifies this, footprint
+    {
+        expirayDate := newExpirayDate;
+    }
+
+    method isExpiredDate(currentDate: int) returns(expired: bool) 
+    requires ValidBB()
+    requires currentDate >= 0
+    ensures ValidBB()
+    ensures expirayDate <= currentDate ==> expired == true
+    ensures fresh(footprint - old(footprint))
+    modifies this, footprint
+    {
+        if (expirayDate <= currentDate) {
+            expired := false;
         }
+        expired := true;
     }
 }
+
+
