dafny/project/BloodType.dfy
@@ -1,34 +1,34 @@
-module BT {
-    import A = BB
-    class BloodType 
+datatype BB = BloodBags 
+datatype Tree<T> = Leaf(T) | Node1(T, Tree<T>) | Node2(T, Tree<T>, Tree<T>)
+class BloodType 
+{
+    ghost var footprint: set<object>;
+    var bloodType: string;
+    var lowest: int;
+    var quantity: int;
+    var listOfBloodBag: array<BB>:= new BB[4]
+
+    predicate ValidBT()
+    reads this, BloodBags
     {
+        {this, listOfBloodBags} <= footprint &&
+        listOfBloodBags.footprint <= footprint &&
+        this !in listOfBloodBags.footprint &&
+        listOfBloodBags.ValidBB() &&
+        lowest >= 0 &&
+        quantity >= 0 &&
+        (bloodType == 'A' || bloodType == 'B' || bloodType == 'O') 
+    }
 
-        var bloodType: string;
-        var lowest: int;
-        var quantity: int;
-        var listOfBloodBags: BloodBags;
-
-        predicate ValidBT()
-        reads this, BloodBags
-        {
-            lowest >= 0 &&
-            quantity >= 0 &&
-            (bloodType == 'A' || bloodType == 'B' || bloodType == 'O') 
-        }
-
-        constructor(bloodtype: string, critical: int)
-        ensures ValidBT()
-        ensures fresh(listOfBloodBags)
-        modifies this, BloodBags
-        {
-            var temp1 := new BloodBags;
-            
-            bloodType := bloodtype;
-            lowest := critical;
-            //listOfBloodBags := array<A> := new A[10];
-            quantity := 0;
-        }
-        A.BloodBags(1, "A", 1, "12/12/12", "12/12/12");
-        
+    constructor()
+    ensures ValidBT()
+    ensures fresh(listOfBloodBags)
+    modifies this, BloodBags
+    {
+        var temp1 := new BloodBags();
+        listOfBloodBags := temp1;
+        bloodType := bloodtype;
+        lowest := critical;
+        quantity := 0;
     }
 }
