dafny/project/BloodTypeReal.dfy
@@ -1,0 +1,2 @@
+datatype BloodType<B> = BloodBags | Node1(B, BloodType<B>)
+predicate ()
